ExistentialRules/Terms/Cyclic.lean
@@ -1,207 +1,227 @@
 import ExistentialRules.Terms.Basic
 
-variable {sig : Signature} [DecidableEq sig.V]
+/-!
+# Cyclic Terms
+
+In this file, we define when a `PreGroundTerm` is `cyclic`.
+This is exactly the case, when a function symbol contains twice in a nested fashion.
+For example $h(d, f(g(f(c))))$ is cyclic but $h(f(d), f(c))$ is not.
+Cyclic terms are mainly used to define MFA later.
+
+The main result in this file then is `cyclic_of_depth_too_big`. That is, if a term exceeds a certain depth, then it is necessarily cyclic.
+This of course requires that only finitely many different function symbols are usable.
+-/
 
 namespace PreGroundTerm
 
-  def function_paths : FiniteTree (SkolemFS sig) sig.C -> List (List (SkolemFS sig))
-  | .leaf _ => [[]]
-  | .inner f ts =>
-    if ts = [] then [[f]] else
-    (ts.flatMap function_paths).map (fun path => f :: path)
+variable {sig : Signature} [DecidableEq sig.V]
 
-  theorem function_path_elements_are_inner_labels (t : FiniteTree (SkolemFS sig) sig.C) : ∀ (path : List (SkolemFS sig)), path ∈ PreGroundTerm.function_paths t -> ∀f, f ∈ path -> f ∈ t.innerLabels := by
-    intro path path_mem f f_mem
-    induction t generalizing path with
-    | leaf c =>
-      simp only [function_paths, List.mem_singleton] at path_mem
+/-- The `function_paths` of a `PreGroundTerm` are essentially all the (maximal) branches in the underlying finite tree without the terminal constant symbol. These can be used to detect cyclic terms by simply looking for repetitions along a branch. -/
+def function_paths : FiniteTree (SkolemFS sig) sig.C -> List (List (SkolemFS sig))
+| .leaf _ => [[]]
+| .inner f ts =>
+  if ts = [] then [[f]] else
+  (ts.flatMap function_paths).map (fun path => f :: path)
+
+/-- A `PreGroundTerm` contains a function symbol if this symbols occurs as one of the inner labels. -/
+def contains_func (func : SkolemFS sig) : FiniteTree (SkolemFS sig) sig.C -> Bool
+| .leaf _ => false
+| .inner func' ts => func == func' || ts.attach.any (fun ⟨t, _⟩ => contains_func func t)
+
+/-- A `PreGroundTerm` is `cyclic` if one of its children `contains_func` the function symbol of the term or if one of its children is already `cyclic`. Constants are never cyclic. -/
+def cyclic : FiniteTree (SkolemFS sig) sig.C -> Bool
+| .leaf _ => false
+| .inner func ts => ts.any (contains_func func) || ts.attach.any (fun ⟨t, _⟩ => PreGroundTerm.cyclic t)
+
+/-- All elements of the `function_paths` paths are inner labels of the finite tree. -/
+theorem function_path_elements_are_inner_labels (t : FiniteTree (SkolemFS sig) sig.C) : ∀ (path : List (SkolemFS sig)), path ∈ PreGroundTerm.function_paths t -> ∀f, f ∈ path -> f ∈ t.innerLabels := by
+  intro path path_mem f f_mem
+  induction t generalizing path with
+  | leaf c =>
+    simp only [function_paths, List.mem_singleton] at path_mem
+    rw [path_mem] at f_mem
+    simp at f_mem
+  | inner func ts ih =>
+    unfold function_paths at path_mem
+    cases ts with
+    | nil =>
+      simp only [↓reduceIte] at path_mem
+      rw [List.mem_singleton] at path_mem
       rw [path_mem] at f_mem
-      simp at f_mem
-    | inner func ts ih =>
-      unfold function_paths at path_mem
-      cases ts with
-      | nil =>
-        simp only [↓reduceIte] at path_mem
-        rw [List.mem_singleton] at path_mem
-        rw [path_mem] at f_mem
-        rw [List.mem_singleton] at f_mem
-        unfold FiniteTree.innerLabels
-        rw [List.mem_cons]
-        apply Or.inl
-        exact f_mem
-      | cons hd tl =>
-        simp only [List.cons_ne_nil, ↓reduceIte] at path_mem
-        rw [List.map_flatMap, List.mem_flatMap] at path_mem
-        rcases path_mem with ⟨t, t_mem, path_mem⟩
-        rw [List.mem_map] at path_mem
-        rcases path_mem with ⟨path', mem, eq⟩
-        rw [← eq] at f_mem
-        rw [List.mem_cons] at f_mem
-        unfold FiniteTree.innerLabels
-        rw [List.mem_cons]
-        cases f_mem with
-        | inl f_mem => apply Or.inl; exact f_mem
-        | inr f_mem =>
-          apply Or.inr
-          rw [List.mem_flatMap]
-          exists t
-          constructor
-          . exact t_mem
-          . exact ih t t_mem path' mem f_mem
-
-  theorem function_path_of_depth_exists (t : FiniteTree (SkolemFS sig) sig.C) : ∃ (path : List (SkolemFS sig)), path ∈ PreGroundTerm.function_paths t ∧ path.length = t.depth - 1 := by
-    induction t with
-    | leaf c => exists []; simp [FiniteTree.depth, function_paths]
-    | inner f ts ih =>
-      cases ts with
-      | nil =>
-        exists [f]
+      rw [List.mem_singleton] at f_mem
+      unfold FiniteTree.innerLabels
+      rw [List.mem_cons]
+      apply Or.inl
+      exact f_mem
+    | cons hd tl =>
+      simp only [List.cons_ne_nil, ↓reduceIte] at path_mem
+      rw [List.map_flatMap, List.mem_flatMap] at path_mem
+      rcases path_mem with ⟨t, t_mem, path_mem⟩
+      rw [List.mem_map] at path_mem
+      rcases path_mem with ⟨path', mem, eq⟩
+      rw [← eq] at f_mem
+      rw [List.mem_cons] at f_mem
+      unfold FiniteTree.innerLabels
+      rw [List.mem_cons]
+      cases f_mem with
+      | inl f_mem => apply Or.inl; exact f_mem
+      | inr f_mem =>
+        apply Or.inr
+        rw [List.mem_flatMap]
+        exists t
         constructor
-        . unfold function_paths
-          simp
-        . unfold FiniteTree.depth
-          simp
-      | cons hd tl =>
-        have : ∃ t, t ∈ (hd::tl) ∧ t.depth = (FiniteTree.inner f (hd :: tl)).depth - 1 := by
-          simp only [FiniteTree.depth]
-          rw [Nat.add_comm, Nat.add_one_sub_one]
-          rw [← List.mem_map]
-          apply List.max?_mem
-          simp
-        rcases this with ⟨t, t_mem, t_depth⟩
-        rcases ih t t_mem with ⟨path, mem, len⟩
-        exists (f :: path)
-        constructor
-        . unfold function_paths
-          simp only [List.cons_ne_nil, ↓reduceIte]
-          rw [List.mem_map]
-          exists path
-          constructor
-          . rw [List.mem_flatMap]
-            exists t
-          . rfl
-        . rw [← t_depth, List.length_cons]
-          rw [len]
-          rw [Nat.sub_one_add_one]
-          intro contra
-          cases t with
-          | leaf _ => simp [FiniteTree.depth] at contra
-          | inner _ _ => simp [FiniteTree.depth] at contra
+        . exact t_mem
+        . exact ih t t_mem path' mem f_mem
 
-  def contains_func (func : SkolemFS sig) : FiniteTree (SkolemFS sig) sig.C -> Bool
-  | .leaf _ => false
-  | .inner func' ts => func == func' || ts.attach.any (fun ⟨t, _⟩ => contains_func func t)
-
-  theorem function_path_elements_are_in_contains_func (t : FiniteTree (SkolemFS sig) sig.C) : ∀ (path : List (SkolemFS sig)), path ∈ PreGroundTerm.function_paths t -> ∀ f, f ∈ path -> PreGroundTerm.contains_func f t := by
-    intro path path_mem f f_mem
-    induction t generalizing path with
-    | leaf c =>
-      simp only [function_paths, List.mem_singleton] at path_mem
-      rw [path_mem] at f_mem
-      simp at f_mem
-    | inner func ts ih =>
-      unfold contains_func
-      rw [Bool.or_eq_true]
-      unfold function_paths at path_mem
-      cases ts with
-      | nil =>
-        simp only [↓reduceIte] at path_mem
-        rw [List.mem_singleton] at path_mem
-        rw [path_mem] at f_mem
-        rw [List.mem_singleton] at f_mem
-        apply Or.inl
-        rw [f_mem]
+/-- There is a path in `function_paths` that matches the depth of the term (-1). That means that this path is one of maximal possible length. -/
+theorem function_path_of_depth_exists (t : FiniteTree (SkolemFS sig) sig.C) : ∃ (path : List (SkolemFS sig)), path ∈ PreGroundTerm.function_paths t ∧ path.length = t.depth - 1 := by
+  induction t with
+  | leaf c => exists []; simp [FiniteTree.depth, function_paths]
+  | inner f ts ih =>
+    cases ts with
+    | nil =>
+      exists [f]
+      constructor
+      . unfold function_paths
         simp
-      | cons hd tl =>
-        simp only [List.cons_ne_nil, ↓reduceIte] at path_mem
-        rw [List.map_flatMap, List.mem_flatMap] at path_mem
-        rcases path_mem with ⟨t, t_mem, path_mem⟩
-        rw [List.mem_map] at path_mem
-        rcases path_mem with ⟨path', mem, eq⟩
-        rw [← eq] at f_mem
-        rw [List.mem_cons] at f_mem
-        cases f_mem with
-        | inl f_mem => apply Or.inl; rw [f_mem]; simp
-        | inr f_mem =>
-          apply Or.inr
-          rw [List.any_eq_true]
-          exists ⟨t, t_mem⟩
-          constructor
-          . apply List.mem_attach
-          . exact ih t t_mem path' mem f_mem
+      . unfold FiniteTree.depth
+        simp
+    | cons hd tl =>
+      have : ∃ t, t ∈ (hd::tl) ∧ t.depth = (FiniteTree.inner f (hd :: tl)).depth - 1 := by
+        simp only [FiniteTree.depth]
+        rw [Nat.add_comm, Nat.add_one_sub_one]
+        rw [← List.mem_map]
+        apply List.max?_mem
+        simp
+      rcases this with ⟨t, t_mem, t_depth⟩
+      rcases ih t t_mem with ⟨path, mem, len⟩
+      exists (f :: path)
+      constructor
+      . unfold function_paths
+        simp only [List.cons_ne_nil, ↓reduceIte]
+        rw [List.mem_map]
+        exists path
+        constructor
+        . rw [List.mem_flatMap]
+          exists t
+        . rfl
+      . rw [← t_depth, List.length_cons]
+        rw [len]
+        rw [Nat.sub_one_add_one]
+        intro contra
+        cases t with
+        | leaf _ => simp [FiniteTree.depth] at contra
+        | inner _ _ => simp [FiniteTree.depth] at contra
 
-  def cyclic : FiniteTree (SkolemFS sig) sig.C -> Bool
-  | .leaf _ => false
-  | .inner func ts => ts.any (contains_func func) || ts.attach.any (fun ⟨t, _⟩ => PreGroundTerm.cyclic t)
+/-- For each element in a path from `function_paths`, `contains_func` is true. -/
+theorem function_path_elements_are_in_contains_func (t : FiniteTree (SkolemFS sig) sig.C) : ∀ (path : List (SkolemFS sig)), path ∈ PreGroundTerm.function_paths t -> ∀ f, f ∈ path -> PreGroundTerm.contains_func f t := by
+  intro path path_mem f f_mem
+  induction t generalizing path with
+  | leaf c =>
+    simp only [function_paths, List.mem_singleton] at path_mem
+    rw [path_mem] at f_mem
+    simp at f_mem
+  | inner func ts ih =>
+    unfold contains_func
+    rw [Bool.or_eq_true]
+    unfold function_paths at path_mem
+    cases ts with
+    | nil =>
+      simp only [↓reduceIte] at path_mem
+      rw [List.mem_singleton] at path_mem
+      rw [path_mem] at f_mem
+      rw [List.mem_singleton] at f_mem
+      apply Or.inl
+      rw [f_mem]
+      simp
+    | cons hd tl =>
+      simp only [List.cons_ne_nil, ↓reduceIte] at path_mem
+      rw [List.map_flatMap, List.mem_flatMap] at path_mem
+      rcases path_mem with ⟨t, t_mem, path_mem⟩
+      rw [List.mem_map] at path_mem
+      rcases path_mem with ⟨path', mem, eq⟩
+      rw [← eq] at f_mem
+      rw [List.mem_cons] at f_mem
+      cases f_mem with
+      | inl f_mem => apply Or.inl; rw [f_mem]; simp
+      | inr f_mem =>
+        apply Or.inr
+        rw [List.any_eq_true]
+        exists ⟨t, t_mem⟩
+        constructor
+        . apply List.mem_attach
+        . exact ih t t_mem path' mem f_mem
 
-  theorem cyclic_of_path_with_dup (t : FiniteTree (SkolemFS sig) sig.C) (path : List (SkolemFS sig)) (path_mem : path ∈ PreGroundTerm.function_paths t) (dup : ¬ path.Nodup) : PreGroundTerm.cyclic t := by
-    induction t generalizing path with
-    | leaf c =>
-      unfold PreGroundTerm.function_paths at path_mem
+/-- A term is `cyclic` if a path in `function_paths` has a duplicate. -/
+theorem cyclic_of_path_with_dup (t : FiniteTree (SkolemFS sig) sig.C) (path : List (SkolemFS sig)) (path_mem : path ∈ PreGroundTerm.function_paths t) (dup : ¬ path.Nodup) : PreGroundTerm.cyclic t := by
+  induction t generalizing path with
+  | leaf c =>
+    unfold PreGroundTerm.function_paths at path_mem
+    rw [List.mem_singleton] at path_mem
+    rw [path_mem] at dup
+    simp at dup
+  | inner f ts ih =>
+    unfold PreGroundTerm.function_paths at path_mem
+    cases ts with
+    | nil =>
+      simp only [↓reduceIte] at path_mem
       rw [List.mem_singleton] at path_mem
       rw [path_mem] at dup
       simp at dup
-    | inner f ts ih =>
-      unfold PreGroundTerm.function_paths at path_mem
-      cases ts with
-      | nil =>
-        simp only [↓reduceIte] at path_mem
-        rw [List.mem_singleton] at path_mem
-        rw [path_mem] at dup
-        simp at dup
-      | cons hd tl =>
-        simp only [List.cons_ne_nil, ↓reduceIte] at path_mem
-        rw [List.map_flatMap, List.mem_flatMap] at path_mem
-        rcases path_mem with ⟨t, t_mem, path_mem⟩
-        rw [List.mem_map] at path_mem
-        rcases path_mem with ⟨path', mem, eq⟩
-        unfold PreGroundTerm.cyclic
-        rw [Bool.or_eq_true]
-        cases Decidable.em (f ∈ path') with
-        | inl f_mem =>
-          apply Or.inl
-          rw [List.any_eq_true]
-          exists t
-          constructor
-          . exact t_mem
-          . exact function_path_elements_are_in_contains_func t path' mem f f_mem
-        | inr f_mem =>
-          apply Or.inr
-          rw [← eq] at dup
-          rw [List.nodup_cons] at dup
-          simp only [not_and] at dup
-          rw [List.any_eq_true]
-          exists ⟨t, t_mem⟩
-          constructor
-          . apply List.mem_attach
-          . exact ih t t_mem path' mem (dup f_mem)
+    | cons hd tl =>
+      simp only [List.cons_ne_nil, ↓reduceIte] at path_mem
+      rw [List.map_flatMap, List.mem_flatMap] at path_mem
+      rcases path_mem with ⟨t, t_mem, path_mem⟩
+      rw [List.mem_map] at path_mem
+      rcases path_mem with ⟨path', mem, eq⟩
+      unfold PreGroundTerm.cyclic
+      rw [Bool.or_eq_true]
+      cases Decidable.em (f ∈ path') with
+      | inl f_mem =>
+        apply Or.inl
+        rw [List.any_eq_true]
+        exists t
+        constructor
+        . exact t_mem
+        . exact function_path_elements_are_in_contains_func t path' mem f f_mem
+      | inr f_mem =>
+        apply Or.inr
+        rw [← eq] at dup
+        rw [List.nodup_cons] at dup
+        simp only [not_and] at dup
+        rw [List.any_eq_true]
+        exists ⟨t, t_mem⟩
+        constructor
+        . apply List.mem_attach
+        . exact ih t t_mem path' mem (dup f_mem)
 
 
-  variable [DecidableEq sig.C]
+variable [DecidableEq sig.C]
 
-  theorem cyclic_of_depth_too_big (t : PreGroundTerm sig) (funcs : List (SkolemFS sig)) (nodup : funcs.Nodup) (funcs_in_t_from_funcs : ∀ func, func ∈ t.innerLabels -> func ∈ funcs) : funcs.length + 2 ≤ t.depth -> PreGroundTerm.cyclic t := by
-    intro le_depth
-    have := PreGroundTerm.function_path_of_depth_exists t
-    rcases this with ⟨path, path_mem, path_len⟩
+/-- Consider a (deduplicated) list of possible function symbols and a term. If the depth of the term is at least the number of function symbols + 2, then the term must be cyclic.  -/
+theorem cyclic_of_depth_too_big (t : PreGroundTerm sig) (funcs : List (SkolemFS sig)) (nodup : funcs.Nodup) (funcs_in_t_from_funcs : ∀ func, func ∈ t.innerLabels -> func ∈ funcs) : funcs.length + 2 ≤ t.depth -> PreGroundTerm.cyclic t := by
+  intro le_depth
+  have := PreGroundTerm.function_path_of_depth_exists t
+  rcases this with ⟨path, path_mem, path_len⟩
 
-    have path_length_gt : funcs.length < path.length := by
-      rw [path_len]
-      apply Nat.lt_of_succ_le
-      apply Nat.le_of_succ_le_succ
-      rw [Nat.succ_eq_add_one]
-      rw [Nat.succ_eq_add_one]
-      rw [Nat.sub_one_add_one]
-      . exact le_depth
-      . unfold FiniteTree.depth
-        cases t <;> simp
+  have path_length_gt : funcs.length < path.length := by
+    rw [path_len]
+    apply Nat.lt_of_succ_le
+    apply Nat.le_of_succ_le_succ
+    rw [Nat.succ_eq_add_one]
+    rw [Nat.succ_eq_add_one]
+    rw [Nat.sub_one_add_one]
+    . exact le_depth
+    . unfold FiniteTree.depth
+      cases t <;> simp
 
-    have dup_in_path : ¬ path.Nodup := by
-      apply List.contains_dup_of_exceeding_nodup_list_with_same_elements funcs path nodup path_length_gt
-      intro f f_mem
-      apply funcs_in_t_from_funcs
-      exact PreGroundTerm.function_path_elements_are_inner_labels t path path_mem f f_mem
+  have dup_in_path : ¬ path.Nodup := by
+    apply List.contains_dup_of_exceeding_nodup_list_with_same_elements funcs path nodup path_length_gt
+    intro f f_mem
+    apply funcs_in_t_from_funcs
+    exact PreGroundTerm.function_path_elements_are_inner_labels t path path_mem f f_mem
 
-    exact PreGroundTerm.cyclic_of_path_with_dup t path path_mem dup_in_path
+  exact PreGroundTerm.cyclic_of_path_with_dup t path path_mem dup_in_path
 
 end PreGroundTerm
 
